[C$] Abbreviate some names.

books/kestrel/c/syntax/preprocessor-states.lisp
@@ -414,7 +414,7 @@
 
 ;;;;;;;;;;;;;;;;;;;;;;;;;;;;;;;;;;;;;;;;;;;;;;;;;;;;;;;;;;;;;;;;;;;;;;;;;;;;;;;;
 
-(fty::deftagsum lexeme/marker
+(fty::deftagsum lexmark
   :short "Fixtype of preprocessing lexemes and markers."
   :long
   (xdoc::topstring
@@ -437,37 +437,37 @@
   (:start ((macro ident)))
   (:end ((macro ident)))
   (:placemarker ())
-  :pred lexeme/marker-p)
+  :pred lexmarkp)
 
 ;;;;;;;;;;;;;;;;;;;;
 
-(defirrelevant irr-lexeme/marker
+(defirrelevant irr-lexmark
   :short "An irrelevant preprocessing lexeme or marker."
-  :type lexeme/marker-p
-  :body (lexeme/marker-lexeme (irr-plexeme+span)))
+  :type lexmarkp
+  :body (lexmark-lexeme (irr-plexeme+span)))
 
 ;;;;;;;;;;;;;;;;;;;;;;;;;;;;;;;;;;;;;;;;
 
-(fty::deflist lexeme/marker-list
+(fty::deflist lexmark-list
   :short "Fixtype of lists of preprocessing lexemes and markers."
-  :elt-type lexeme/marker
+  :elt-type lexmark
   :true-listp t
   :elementp-of-nil nil
-  :pred lexeme/marker-listp
+  :pred lexmark-listp
 
   ///
 
-  (defruled lexeme/marker-listp-of-resize-list
-    (implies (and (lexeme/marker-listp lexmarks)
-                  (lexeme/marker-p default))
-             (lexeme/marker-listp (resize-list lexmarks length default)))
+  (defruled lexmark-listp-of-resize-list
+    (implies (and (lexmark-listp lexmarks)
+                  (lexmarkp default))
+             (lexmark-listp (resize-list lexmarks length default)))
     :induct t
     :enable (resize-list))
 
-  (defruled lexeme/marker-listp-of-update-nth-strong
-    (implies (lexeme/marker-listp lexmarks)
-             (equal (lexeme/marker-listp (update-nth i lexmark lexmarks))
-                    (and (lexeme/marker-p lexmark)
+  (defruled lexmark-listp-of-update-nth-strong
+    (implies (lexmark-listp lexmarks)
+             (equal (lexmark-listp (update-nth i lexmark lexmarks))
+                    (and (lexmarkp lexmark)
                          (<= (nfix i) (len lexmarks)))))
     :induct t
     :enable (update-nth nfix zp len)))
@@ -906,66 +906,64 @@
                   :initially 0)
       (chars-unread :type (integer 0 *)
                     :initially 0)
-      (lexemes/markers :type (array (satisfies lexeme/marker-p) (1))
-                      :initially ,(irr-lexeme/marker)
-                      :resizable t)
-      (lexemes/markers-read :type (integer 0 *)
-                           :initially 0)
-      (lexemes/markers-unread :type (integer 0 *)
-                             :initially 0)
+      (lexmarks :type (array (satisfies lexmarkp) (1))
+                :initially ,(irr-lexmark)
+                :resizable t)
+      (lexmarks-read :type (integer 0 *)
+                     :initially 0)
+      (lexmarks-unread :type (integer 0 *)
+                       :initially 0)
       (ienv :type (satisfies ienvp)
             :initially ,(irr-ienv))
       (size :type (integer 0 *)
             :initially 0)
       (macros :type (satisfies macro-tablep)
               :initially ,(macro-table-init))
-      :renaming
-      (;; field recognizers:
-       (bytessp raw-ppstate->bytess-p)
-       (bytess-currentp raw-ppstate->bytess-current-p)
-       (positionp raw-ppstate->position-p)
-       (charsp raw-ppstate->chars-p)
-       (chars-readp raw-ppstate->chars-read-p)
-       (chars-unreadp raw-ppstate->chars-unread-p)
-       (lexemes/markersp raw-ppstate->lexemes/markers-p)
-       (lexemes/markers-readp raw-ppstate->lexemes/markers-read-p)
-       (lexemes/markers-unreadp raw-ppstate->lexemes/markers-unread-p)
-       (ienvp raw-ppstate->ienvp)
-       (sizep raw-ppstate->size-p)
-       (macrosp raw-ppstate->macros-p)
-       ;; field readers:
-       (bytess-length raw-ppstate->bytess-length)
-       (bytessi raw-ppstate->bytes)
-       (bytess-current raw-ppstate->bytess-current)
-       (position raw-ppstate->position)
-       (chars-length raw-ppstate->chars-length)
-       (charsi raw-ppstate->char)
-       (chars-read raw-ppstate->chars-read)
-       (chars-unread raw-ppstate->chars-unread)
-       (lexemes/markers-length raw-ppstate->lexemes/markers-length)
-       (lexemes/markersi raw-ppstate->lexeme/marker)
-       (lexemes/markers-read raw-ppstate->lexemes/markers-read)
-       (lexemes/markers-unread raw-ppstate->lexemes/markers-unread)
-       (ienv raw-ppstate->ienv)
-       (size raw-ppstate->size)
-       (macros raw-ppstate->macros)
-       ;; field writers:
-       (resize-bytess raw-update-ppstate->bytess-length)
-       (update-bytessi raw-update-ppstate->bytes)
-       (update-bytess-current raw-update-ppstate->bytess-current)
-       (update-position raw-update-ppstate->position)
-       (resize-chars raw-update-ppstate->chars-length)
-       (update-charsi raw-update-ppstate->char)
-       (update-chars-read raw-update-ppstate->chars-read)
-       (update-chars-unread raw-update-ppstate->chars-unread)
-       (resize-lexemes/markers raw-update-ppstate->lexemes/markers-length)
-       (update-lexemes/markersi raw-update-ppstate->lexeme/marker)
-       (update-lexemes/markers-read raw-update-ppstate->lexemes/markers-read)
-       (update-lexemes/markers-unread
-        raw-update-ppstate->lexemes/markers-unread)
-       (update-ienv raw-update-ppstate->ienv)
-       (update-size raw-update-ppstate->size)
-       (update-macros raw-update-ppstate->macros))))
+      :renaming (;; field recognizers:
+                 (bytessp raw-ppstate->bytess-p)
+                 (bytess-currentp raw-ppstate->bytess-current-p)
+                 (positionp raw-ppstate->position-p)
+                 (charsp raw-ppstate->chars-p)
+                 (chars-readp raw-ppstate->chars-read-p)
+                 (chars-unreadp raw-ppstate->chars-unread-p)
+                 (lexmarksp raw-ppstate->lexmarks-p)
+                 (lexmarks-readp raw-ppstate->lexmarks-read-p)
+                 (lexmarks-unreadp raw-ppstate->lexmarks-unread-p)
+                 (ienvp raw-ppstate->ienvp)
+                 (sizep raw-ppstate->size-p)
+                 (macrosp raw-ppstate->macros-p)
+                 ;; field readers:
+                 (bytess-length raw-ppstate->bytess-length)
+                 (bytessi raw-ppstate->bytes)
+                 (bytess-current raw-ppstate->bytess-current)
+                 (position raw-ppstate->position)
+                 (chars-length raw-ppstate->chars-length)
+                 (charsi raw-ppstate->char)
+                 (chars-read raw-ppstate->chars-read)
+                 (chars-unread raw-ppstate->chars-unread)
+                 (lexmarks-length raw-ppstate->lexmarks-length)
+                 (lexmarksi raw-ppstate->lexmark)
+                 (lexmarks-read raw-ppstate->lexmarks-read)
+                 (lexmarks-unread raw-ppstate->lexmarks-unread)
+                 (ienv raw-ppstate->ienv)
+                 (size raw-ppstate->size)
+                 (macros raw-ppstate->macros)
+                 ;; field writers:
+                 (resize-bytess raw-update-ppstate->bytess-length)
+                 (update-bytessi raw-update-ppstate->bytes)
+                 (update-bytess-current raw-update-ppstate->bytess-current)
+                 (update-position raw-update-ppstate->position)
+                 (resize-chars raw-update-ppstate->chars-length)
+                 (update-charsi raw-update-ppstate->char)
+                 (update-chars-read raw-update-ppstate->chars-read)
+                 (update-chars-unread raw-update-ppstate->chars-unread)
+                 (resize-lexmarks raw-update-ppstate->lexmarks-length)
+                 (update-lexmarksi raw-update-ppstate->lexmark)
+                 (update-lexmarks-read raw-update-ppstate->lexmarks-read)
+                 (update-lexmarks-unread raw-update-ppstate->lexmarks-unread)
+                 (update-ienv raw-update-ppstate->ienv)
+                 (update-size raw-update-ppstate->size)
+                 (update-macros raw-update-ppstate->macros))))
 
   ;; fixer:
 
@@ -1006,12 +1004,12 @@
     :enable (raw-ppstate->chars-p
              char+position-listp))
 
-  (defrule raw-ppstate->lexemes/markers-p-becomes-lexeme/marker-listp
-    (equal (raw-ppstate->lexemes/markers-p x)
-           (lexeme/marker-listp x))
+  (defrule raw-ppstate->lexmarks-p-becomes-lexmark-listp
+    (equal (raw-ppstate->lexmarks-p x)
+           (lexmark-listp x))
     :induct t
-    :enable (raw-ppstate->lexemes/markers-p
-             lexeme/marker-listp))
+    :enable (raw-ppstate->lexmarks-p
+             lexmark-listp))
 
   ;; needed for reader/writer proofs:
 
@@ -1089,43 +1087,43 @@
                   0)
          :exec (raw-ppstate->chars-unread ppstate)))
 
-  (define ppstate->lexemes/markers-length (ppstate)
+  (define ppstate->lexmarks-length (ppstate)
     :returns (length natp)
     (mbe :logic (if (ppstatep ppstate)
-                    (raw-ppstate->lexemes/markers-length ppstate)
+                    (raw-ppstate->lexmarks-length ppstate)
                   1)
-         :exec (raw-ppstate->lexemes/markers-length ppstate)))
+         :exec (raw-ppstate->lexmarks-length ppstate)))
 
-  (define ppstate->lexeme/marker ((i natp) ppstate)
-    :guard (< i (ppstate->lexemes/markers-length ppstate))
-    :returns (lexeme/marker lexeme/marker-p
-                     :hints
-                     (("Goal"
-                       :in-theory (enable ppstate->lexemes/markers-length))))
+  (define ppstate->lexmark ((i natp) ppstate)
+    :guard (< i (ppstate->lexmarks-length ppstate))
+    :returns (lexmark lexmarkp
+                      :hints
+                      (("Goal"
+                        :in-theory (enable ppstate->lexmarks-length))))
     (mbe :logic (if (and (ppstatep ppstate)
-                         (< (nfix i) (ppstate->lexemes/markers-length ppstate)))
-                    (raw-ppstate->lexeme/marker (nfix i) ppstate)
-                  (irr-lexeme/marker))
-         :exec (raw-ppstate->lexeme/marker i ppstate))
+                         (< (nfix i) (ppstate->lexmarks-length ppstate)))
+                    (raw-ppstate->lexmark (nfix i) ppstate)
+                  (irr-lexmark))
+         :exec (raw-ppstate->lexmark i ppstate))
     :guard-hints
-    (("Goal" :in-theory (enable nfix ppstate->lexemes/markers-length)))
+    (("Goal" :in-theory (enable nfix ppstate->lexmarks-length)))
     :hooks nil)
 
-  (define ppstate->lexemes/markers-read (ppstate)
-    :returns (lexemes/markers-read natp
-                                  :rule-classes (:rewrite :type-prescription))
+  (define ppstate->lexmarks-read (ppstate)
+    :returns (lexmarks-read natp
+                            :rule-classes (:rewrite :type-prescription))
     (mbe :logic (if (ppstatep ppstate)
-                    (raw-ppstate->lexemes/markers-read ppstate)
+                    (raw-ppstate->lexmarks-read ppstate)
                   0)
-         :exec (raw-ppstate->lexemes/markers-read ppstate)))
+         :exec (raw-ppstate->lexmarks-read ppstate)))
 
-  (define ppstate->lexemes/markers-unread (ppstate)
-    :returns (lexemes/markers-unread natp
-                                    :rule-classes (:rewrite :type-prescription))
+  (define ppstate->lexmarks-unread (ppstate)
+    :returns (lexmarks-unread natp
+                              :rule-classes (:rewrite :type-prescription))
     (mbe :logic (if (ppstatep ppstate)
-                    (raw-ppstate->lexemes/markers-unread ppstate)
+                    (raw-ppstate->lexmarks-unread ppstate)
                   0)
-         :exec (raw-ppstate->lexemes/markers-unread ppstate)))
+         :exec (raw-ppstate->lexmarks-unread ppstate)))
 
   (define ppstate->ienv (ppstate)
     :returns (ienv ienvp)
@@ -1233,52 +1231,52 @@
     (b* ((ppstate (ppstate-fix ppstate)))
       (raw-update-ppstate->chars-unread (lnfix chars-unread) ppstate)))
 
-  (define update-ppstate->lexemes/markers-length ((length natp) ppstate)
+  (define update-ppstate->lexmarks-length ((length natp) ppstate)
     :returns (ppstate ppstatep
                       :hints
                       (("Goal"
                         :in-theory
                         (enable nfix
                                 length
-                                lexeme/marker-listp-of-resize-list))))
+                                lexmark-listp-of-resize-list))))
     (b* ((ppstate (ppstate-fix ppstate)))
-      (raw-update-ppstate->lexemes/markers-length (lnfix length) ppstate)))
+      (raw-update-ppstate->lexmarks-length (lnfix length) ppstate)))
 
-  (define update-ppstate->lexeme/marker ((i natp)
-                                         (lexmark lexeme/marker-p)
-                                         ppstate)
-    :guard (< i (ppstate->lexemes/markers-length ppstate))
+  (define update-ppstate->lexmark ((i natp)
+                                   (lexmark lexmarkp)
+                                   ppstate)
+    :guard (< i (ppstate->lexmarks-length ppstate))
     :returns (ppstate ppstatep
                       :hints
                       (("Goal"
                         :in-theory
                         (enable update-nth-array
-                                ppstate->lexemes/markers-length
-                                lexeme/marker-listp-of-update-nth-strong))))
+                                ppstate->lexmarks-length
+                                lexmark-listp-of-update-nth-strong))))
     (b* ((ppstate (ppstate-fix ppstate)))
-      (mbe :logic (if (< (nfix i) (ppstate->lexemes/markers-length ppstate))
-                      (raw-update-ppstate->lexeme/marker (nfix i)
-                                                  (lexeme/marker-fix lexmark)
-                                                  ppstate)
+      (mbe :logic (if (< (nfix i) (ppstate->lexmarks-length ppstate))
+                      (raw-update-ppstate->lexmark (nfix i)
+                                                   (lexmark-fix lexmark)
+                                                   ppstate)
                     ppstate)
-           :exec (raw-update-ppstate->lexeme/marker i lexmark ppstate)))
+           :exec (raw-update-ppstate->lexmark i lexmark ppstate)))
     :guard-hints
-    (("Goal" :in-theory (enable ppstate->lexemes/markers-length nfix)))
+    (("Goal" :in-theory (enable ppstate->lexmarks-length nfix)))
     :hooks nil)
 
-  (define update-ppstate->lexemes/markers-read ((lexemes/markers-read natp)
-                                               ppstate)
+  (define update-ppstate->lexmarks-read ((lexmarks-read natp)
+                                         ppstate)
     :returns (ppstate ppstatep)
     (b* ((ppstate (ppstate-fix ppstate)))
-      (raw-update-ppstate->lexemes/markers-read (lnfix lexemes/markers-read)
-                                               ppstate)))
+      (raw-update-ppstate->lexmarks-read (lnfix lexmarks-read)
+                                         ppstate)))
 
-  (define update-ppstate->lexemes/markers-unread
-    ((lexemes/markers-unread natp) ppstate)
+  (define update-ppstate->lexmarks-unread
+    ((lexmarks-unread natp) ppstate)
     :returns (ppstate ppstatep)
     (b* ((ppstate (ppstate-fix ppstate)))
-      (raw-update-ppstate->lexemes/markers-unread
-       (lnfix lexemes/markers-unread) ppstate)))
+      (raw-update-ppstate->lexmarks-unread
+       (lnfix lexmarks-unread) ppstate)))
 
   (define update-ppstate->ienv ((ienv ienvp) ppstate)
     :returns (ppstate ppstatep)
@@ -1372,11 +1370,11 @@
              ppstatep
              length))
 
-  (defrule ppstate->lexemes/markers-length-of-update-ppstate->bytes
-    (equal (ppstate->lexemes/markers-length
+  (defrule ppstate->lexmarks-length-of-update-ppstate->bytes
+    (equal (ppstate->lexmarks-length
             (update-ppstate->bytes i bytes ppstate))
-           (ppstate->lexemes/markers-length ppstate))
-    :enable (ppstate->lexemes/markers-length
+           (ppstate->lexmarks-length ppstate))
+    :enable (ppstate->lexmarks-length
              update-ppstate->bytes
              ppstatep
              length
@@ -1384,29 +1382,29 @@
              ppstate->bytess-length
              byte-list-listp-of-update-nth-strong))
 
-  (defrule ppstate->lexemes/markers-length-of-update-ppstate->bytess-current
-    (equal (ppstate->lexemes/markers-length
+  (defrule ppstate->lexmarks-length-of-update-ppstate->bytess-current
+    (equal (ppstate->lexmarks-length
             (update-ppstate->bytess-current bytess-current ppstate))
-           (ppstate->lexemes/markers-length ppstate))
-    :enable (ppstate->lexemes/markers-length
+           (ppstate->lexmarks-length ppstate))
+    :enable (ppstate->lexmarks-length
              update-ppstate->bytess-current
              ppstatep
              length))
 
-  (defrule ppstate->lexemes/markers-length-of-update-ppstate->position
-    (equal (ppstate->lexemes/markers-length
+  (defrule ppstate->lexmarks-length-of-update-ppstate->position
+    (equal (ppstate->lexmarks-length
             (update-ppstate->position position ppstate))
-           (ppstate->lexemes/markers-length ppstate))
-    :enable (ppstate->lexemes/markers-length
+           (ppstate->lexmarks-length ppstate))
+    :enable (ppstate->lexmarks-length
              update-ppstate->position
              ppstatep
              length))
 
-  (defrule ppstate->lexemes/markers-length-of-update-ppstate->char
-    (equal (ppstate->lexemes/markers-length
+  (defrule ppstate->lexmarks-length-of-update-ppstate->char
+    (equal (ppstate->lexmarks-length
             (update-ppstate->char i char ppstate))
-           (ppstate->lexemes/markers-length ppstate))
-    :enable (ppstate->lexemes/markers-length
+           (ppstate->lexmarks-length ppstate))
+    :enable (ppstate->lexmarks-length
              update-ppstate->char
              ppstatep
              length
@@ -1414,30 +1412,30 @@
              ppstate->chars-length
              byte-list-listp-of-update-nth-strong))
 
-  (defrule ppstate->lexemes/markers-length-of-update-ppstate->chars-read
-    (equal (ppstate->lexemes/markers-length
+  (defrule ppstate->lexmarks-length-of-update-ppstate->chars-read
+    (equal (ppstate->lexmarks-length
             (update-ppstate->chars-read chars-read ppstate))
-           (ppstate->lexemes/markers-length ppstate))
-    :enable (ppstate->lexemes/markers-length
+           (ppstate->lexmarks-length ppstate))
+    :enable (ppstate->lexmarks-length
              update-ppstate->chars-read
              ppstatep
              length))
 
-  (defrule ppstate->lexemes/markers-length-of-update-ppstate->chars-unread
-    (equal (ppstate->lexemes/markers-length
+  (defrule ppstate->lexmarks-length-of-update-ppstate->chars-unread
+    (equal (ppstate->lexmarks-length
             (update-ppstate->chars-unread chars-unread ppstate))
-           (ppstate->lexemes/markers-length ppstate))
-    :enable (ppstate->lexemes/markers-length
+           (ppstate->lexmarks-length ppstate))
+    :enable (ppstate->lexmarks-length
              update-ppstate->chars-unread
              ppstatep
              length))
 
-  (defrule ppstate->lexemes/markers-length-of-update-ppstate->lexeme/marker
-    (equal (ppstate->lexemes/markers-length
-            (update-ppstate->lexeme/marker i lexeme/marker ppstate))
-           (ppstate->lexemes/markers-length ppstate))
-    :enable (ppstate->lexemes/markers-length
-             update-ppstate->lexeme/marker
+  (defrule ppstate->lexmarks-length-of-update-ppstate->lexmark
+    (equal (ppstate->lexmarks-length
+            (update-ppstate->lexmark i lexmark ppstate))
+           (ppstate->lexmarks-length ppstate))
+    :enable (ppstate->lexmarks-length
+             update-ppstate->lexmark
              ppstatep
              length
              update-nth-array
@@ -1447,31 +1445,31 @@
              len))
 
   (defrule
-    ppstate->lexemes/markers-length-of-update-ppstate->lexemes/markers-read
-    (equal (ppstate->lexemes/markers-length
-            (update-ppstate->lexemes/markers-read lexemes/markers-read ppstate))
-           (ppstate->lexemes/markers-length ppstate))
-    :enable (ppstate->lexemes/markers-length
-             update-ppstate->lexemes/markers-read
+    ppstate->lexmarks-length-of-update-ppstate->lexmarks-read
+    (equal (ppstate->lexmarks-length
+            (update-ppstate->lexmarks-read lexmarks-read ppstate))
+           (ppstate->lexmarks-length ppstate))
+    :enable (ppstate->lexmarks-length
+             update-ppstate->lexmarks-read
              ppstatep
              length))
 
   (defrule
-    ppstate->lexemes/markers-length-of-update-ppstate->lexemes/markers-unread
-    (equal (ppstate->lexemes/markers-length
-            (update-ppstate->lexemes/markers-unread lexemes/markers-unread
-                                                   ppstate))
-           (ppstate->lexemes/markers-length ppstate))
-    :enable (ppstate->lexemes/markers-length
-             update-ppstate->lexemes/markers-unread
+    ppstate->lexmarks-length-of-update-ppstate->lexmarks-unread
+    (equal (ppstate->lexmarks-length
+            (update-ppstate->lexmarks-unread lexmarks-unread
+                                             ppstate))
+           (ppstate->lexmarks-length ppstate))
+    :enable (ppstate->lexmarks-length
+             update-ppstate->lexmarks-unread
              ppstatep
              length))
 
-  (defrule ppstate->lexemes/markers-length-of-update-ppstate->size
-    (equal (ppstate->lexemes/markers-length
+  (defrule ppstate->lexmarks-length-of-update-ppstate->size
+    (equal (ppstate->lexmarks-length
             (update-ppstate->size size ppstate))
-           (ppstate->lexemes/markers-length ppstate))
-    :enable (ppstate->lexemes/markers-length
+           (ppstate->lexmarks-length ppstate))
+    :enable (ppstate->lexmarks-length
              update-ppstate->size
              ppstatep
              length))
@@ -1532,34 +1530,34 @@
              ppstatep
              length))
 
-  (defrule ppstate->size-of-update-ppstate->lexeme/marker
+  (defrule ppstate->size-of-update-ppstate->lexmark
     (equal (ppstate->size
-            (update-ppstate->lexeme/marker i lexeme/marker ppstate))
+            (update-ppstate->lexmark i lexmark ppstate))
            (ppstate->size ppstate))
     :enable (ppstate->size
-             update-ppstate->lexeme/marker
+             update-ppstate->lexmark
              ppstatep
              length
              update-nth-array
-             ppstate->lexemes/markers-length
-             lexeme/marker-listp-of-update-nth-strong))
+             ppstate->lexmarks-length
+             lexmark-listp-of-update-nth-strong))
 
-  (defrule ppstate->size-of-update-ppstate->lexemes/markers-read
+  (defrule ppstate->size-of-update-ppstate->lexmarks-read
     (equal (ppstate->size
-            (update-ppstate->lexemes/markers-read lexemes/markers-read ppstate))
+            (update-ppstate->lexmarks-read lexmarks-read ppstate))
            (ppstate->size ppstate))
     :enable (ppstate->size
-             update-ppstate->lexemes/markers-read
+             update-ppstate->lexmarks-read
              ppstatep
              length))
 
-  (defrule ppstate->size-of-update-ppstate->lexemes/markers-unread
+  (defrule ppstate->size-of-update-ppstate->lexmarks-unread
     (equal (ppstate->size
-            (update-ppstate->lexemes/markers-unread lexemes/markers-unread
-                                                   ppstate))
+            (update-ppstate->lexmarks-unread lexmarks-unread
+                                             ppstate))
            (ppstate->size ppstate))
     :enable (ppstate->size
-             update-ppstate->lexemes/markers-unread
+             update-ppstate->lexmarks-unread
              ppstatep
              length))
 
@@ -1639,9 +1637,9 @@
      The bytes of the file are stored into the first element of the array,
      to which the current byte list index is set to point.
      The position is the initial one.
-     There are no read or unread characters or lexemes/markers.
+     There are no read or unread characters or lexmarks.
      The macro table is obtained by pushing a new scope for the file.
-     We also resize the arrays of characters and lexemes/markers
+     We also resize the arrays of characters and lexmarks
      to the number of data bytes,
      which is overkill but sufficient;
      if this turns out to be too large,
@@ -1656,9 +1654,9 @@
        (ppstate (update-ppstate->chars-length (len data) ppstate))
        (ppstate (update-ppstate->chars-read 0 ppstate))
        (ppstate (update-ppstate->chars-unread 0 ppstate))
-       (ppstate (update-ppstate->lexemes/markers-length (len data) ppstate))
-       (ppstate (update-ppstate->lexemes/markers-read 0 ppstate))
-       (ppstate (update-ppstate->lexemes/markers-unread 0 ppstate))
+       (ppstate (update-ppstate->lexmarks-length (len data) ppstate))
+       (ppstate (update-ppstate->lexmarks-read 0 ppstate))
+       (ppstate (update-ppstate->lexmarks-unread 0 ppstate))
        (ppstate (update-ppstate->ienv ienv ppstate))
        (ppstate (update-ppstate->size (len data) ppstate))
        (ppstate (update-ppstate->macros (macro-table-push macros) ppstate)))
